x86/RawAsmMergeSteps.v
@@ -1,0 +1,393 @@
+Require Import Smallstep.
+Require Import Machregs.
+Require Import Asm.
+Require Import Integers.
+Require Import List.
+Require Import ZArith.
+Require Import Memtype.
+Require Import Memory.
+Require Import Archi.
+Require Import Coqlib.
+Require Import AST.
+Require Import Globalenvs.
+Require Import Events.
+Require Import Values.
+Require Import Conventions1.
+Require Import RawAsm.
+Require Asmgenproof0.
+
+Section WITHMEMORYMODEL.
+
+  Existing Instance mem_accessors_default.
+  Context `{memory_model_ops: Mem.MemoryModelOps}.
+  Context `{external_calls_ops : !ExternalCallsOps mem}.
+  Context `{enable_builtins: !EnableBuiltins mem}.
+
+Section WITHGE.
+  Variable ge : Genv.t Asm.fundef unit.
+
+  Definition pc_at (s: state): option ((function * instruction) + external_function) :=
+    let '(State rs m) := s in
+    match rs PC with
+    | Vptr b o =>
+      match Genv.find_funct_ptr ge b with
+      | Some (Internal f) =>
+        match find_instr (Ptrofs.unsigned o) (fn_code f) with
+        | Some i => Some (inl (f,i))
+        | None => None
+        end
+      | Some (External ef) => Some (inr ef)
+      | None => None
+      end
+    | _ => None
+    end.
+
+  Definition rs_state s :=
+    let '(State rs _) := s in rs.
+
+  Definition m_state s :=
+    let '(State _ m) := s in m.
+
+  Inductive is_call (rs: regset): instruction -> Prop :=
+  | is_call_s:
+      forall symb b sg,
+        Genv.find_symbol ge symb = Some b ->
+        is_call rs (Pcall_s symb sg)
+  | is_call_r:
+      forall (r: ireg) b sg,
+        rs r = Vptr b Ptrofs.zero ->
+        is_call rs (Pcall_r r sg).
+
+  Inductive is_alloc sz : instruction -> Prop :=
+    is_alloc_intro f:
+      frame_size f = sz ->
+      is_alloc sz (Pallocframe f (Ptrofs.sub (Ptrofs.repr (align sz 8)) (Ptrofs.repr (size_chunk Mptr)))).
+
+  Inductive is_free (sz: Z) : instruction -> Prop :=
+    is_free_intro:
+      is_free sz (Pfreeframe sz (Ptrofs.sub (Ptrofs.repr sz) (Ptrofs.repr (size_chunk Mptr)))).
+
+
+  Inductive is_jmp: instruction -> Prop :=
+  | is_jmp_s:
+      forall symb b sg,
+        Genv.find_symbol ge symb = Some b ->
+        is_jmp (Pjmp_s symb sg)
+  | is_jmp_r:
+      forall (r: ireg) sg,
+        is_jmp (Pjmp_r r sg true).
+
+  Inductive step: state -> trace -> state -> Prop :=
+  | step_call_internal:
+      forall s1 s2 s3 f0 icall f ialloc
+        (PC1: pc_at s1 = Some (inl (f0, icall)))
+        (PC2: pc_at s2 = Some (inl (f, ialloc)))
+        (CALL: is_call (rs_state s1) icall)
+        (ALLOC: is_alloc (frame_size (fn_frame f)) ialloc)
+        (STEP1: RawAsm.step ge s1 E0 s2)
+        (STEP2: RawAsm.step ge s2 E0 s3),
+        step s1 E0 s3
+  | step_call_external:
+      forall s1 s2 s3 f0 icall ef t
+        (PC1: pc_at s1 = Some (inl (f0, icall)))
+        (CALL: is_call (rs_state s1) icall)
+        (PC2: pc_at s2 = Some (inr ef))
+        (STEP1: RawAsm.step ge s1 E0 s2)
+        (STEP2: RawAsm.step ge s2 t s3),
+        step s1 t s3
+  | step_free_ret:
+      forall s1 s2 s3 ifree f
+        (PC1: pc_at s1 = Some (inl (f, ifree)))
+        (PC2: pc_at s2 = Some (inl (f, Pret)))
+        (FREE: is_free (frame_size (fn_frame f)) ifree)
+        (STEP1: RawAsm.step ge s1 E0 s2)
+        (STEP2: RawAsm.step ge s2 E0 s3),
+        step s1 E0 s3      
+  | step_free_tailcall:
+      forall s1 s2 s3 s4 ifree ijmp ialloc f0 f
+        (PC1: pc_at s1 = Some (inl (f0, ifree)))
+        (PC2: pc_at s2 = Some (inl (f0, ijmp)))
+        (PC2: pc_at s3 = Some (inl (f, ialloc)))
+        (FREE: is_free (frame_size (fn_frame f0)) ifree)
+        (JMP: is_jmp ijmp)
+        (ALLOC: is_alloc (frame_size (fn_frame f)) ialloc)
+        (STEP1: RawAsm.step ge s1 E0 s2)
+        (STEP2: RawAsm.step ge s2 E0 s3)
+        (STEP3: RawAsm.step ge s3 E0 s4),
+        step s1 E0 s4
+  | step_free_external:
+      forall s1 s2 s3 s4 ifree ijmp f0 ef t
+        (PC1: pc_at s1 = Some (inl (f0, ifree)))
+        (PC2: pc_at s2 = Some (inl (f0, ijmp)))
+        (PC2: pc_at s3 = Some (inr ef))
+        (FREE: is_free (frame_size (fn_frame f0)) ifree)
+        (JMP: is_jmp ijmp)
+        (STEP1: RawAsm.step ge s1 E0 s2)
+        (STEP2: RawAsm.step ge s2 E0 s3)
+        (STEP3: RawAsm.step ge s3 t s4),
+        step s1 t s4
+  | step_other_internal:
+      forall s1 t s2 f0 i
+        (PC: pc_at s1 = Some (inl (f0,i)))
+        (NOFREE: forall f, ~ is_free f i)
+        (NOCALL: ~ is_call (rs_state s1) i)
+        (STEP: RawAsm.step ge s1 t s2),
+        step s1 t s2
+  .
+
+End WITHGE.
+  
+  Definition semantics_gen prog rs m :=
+    Semantics step (initial_state_gen prog rs m) final_state (Genv.globalenv prog).
+
+  Definition semantics prog rs :=
+    Semantics step (initial_state prog rs) final_state (Genv.globalenv prog).
+
+End WITHMEMORYMODEL.
+
+Section SIMU.
+
+  Existing Instance mem_accessors_default.
+  Context `{memory_model_ops: Mem.MemoryModelOps}.
+  Context `{external_calls_ops : !ExternalCallsOps mem}.
+  Context `{enable_builtins: !EnableBuiltins mem}.
+
+  Variable prog: Asm.program.
+  Let ge := Genv.globalenv prog.
+
+  Lemma step_correct:
+    forall s t s' 
+      (STEP : step ge s t s'),
+      plus RawAsm.step (Genv.globalenv prog) s t s'.
+  Proof.
+    intros.
+    inv STEP.
+    - eapply plus_two; eauto.
+    - eapply plus_two; eauto.
+    - eapply plus_two; eauto.
+    - eapply plus_three; eauto.
+    - eapply plus_three; eauto.
+    - apply plus_one; auto.
+  Qed.
+
+  Lemma is_call_dec:
+    forall rs i,
+      is_call ge rs i \/ ~ is_call ge rs i.
+  Proof.
+    destruct i; try now (right; intro A; inv A).
+    - destruct (Genv.find_symbol ge symb) eqn:FS.
+      left; econstructor; eauto.
+      right; intro A; inv A. congruence.
+    - destruct (rs r) eqn:PTR; try now (right; intro A; inv A; congruence).
+      destruct (Ptrofs.eq_dec i Ptrofs.zero). subst.
+      left; econstructor; eauto.
+      right; intro A; inv A; congruence.
+  Qed.
+
+  Lemma is_free_dec:
+    forall i,
+      (exists sz, is_free sz i) \/ ~ exists sz, is_free sz i.
+  Proof.
+    destruct i; try now (right; intro A; inv A).
+    edestruct (Ptrofs.eq_dec ofs_ra). rewrite e.
+    left; exists sz; econstructor; eauto.
+    right; intro A; inv A. inv H. congruence.
+  Qed.
+
+  Inductive is_builtin: instruction -> Prop :=
+  | is_builtin_intro ef args res: is_builtin (Pbuiltin ef args res).
+  
+  Lemma step_internal:
+    forall s t s'
+      (STEP: RawAsm.step ge s t s')
+      f i
+      (PCAT: pc_at ge s = Some (inl (f,i)))
+      (NB: ~ is_builtin i),
+      exec_instr ge f i (rs_state s) (m_state s) = Next (rs_state s') (m_state s') /\ t = E0.
+  Proof.
+    unfold pc_at; intros s t s'  STEP; inv STEP.
+    - rewrite H, H0, H1. inversion 1; subst. simpl. eauto.
+    - rewrite H, H0, H1. intros f0 i A; inv A. intro NIB; exfalso; apply NIB. constructor.
+    - rewrite H, H0. inversion 1.
+  Qed.
+
+  Ltac simpl_regs_in H :=
+    repeat rewrite Pregmap.gso in H by congruence;
+    try rewrite Pregmap.gss in H;
+    try rewrite Asmgenproof0.nextinstr_pc in H.
+
+  Ltac simpl_regs :=
+    repeat rewrite Pregmap.gso by congruence;
+    try rewrite Pregmap.gss;
+    try rewrite Asmgenproof0.nextinstr_pc.
+
+  Record wf_asm_function (f: function): Prop :=
+    {
+      wf_asm_call_target_exists:
+        forall o symb sg,
+          find_instr o (fn_code f) = Some (Pcall_s symb sg) ->
+          exists bf f',
+            Genv.symbol_address ge symb Ptrofs.zero = Vptr bf Ptrofs.zero /\
+            Genv.find_funct_ptr ge bf = Some f';
+      wf_asm_alloc_only_at_beginning:
+        forall o fi ora,
+          find_instr o (fn_code f) = Some (Pallocframe fi ora) ->
+          o = 0;
+      wf_asm_alloc_at_beginning:
+        forall i,
+          find_instr 0 (fn_code f) = Some i ->
+          is_alloc (frame_size (fn_frame f)) i;
+
+      wf_asm_after_freeframe:
+        forall i o sz,
+          find_instr (Ptrofs.unsigned o) (fn_code f) = Some i ->
+          is_free sz i ->
+          sz = frame_size (fn_frame f) /\
+          exists i' ,
+            find_instr (Ptrofs.unsigned (Ptrofs.add o (Ptrofs.repr (instr_size i)))) (fn_code f) = Some i' /\
+            (i' = Pret \/ is_jmp ge i' );
+
+
+    }.
+
+  Hypothesis wf_asm_prog:
+    forall b f,
+      Genv.find_funct_ptr ge b = Some (Internal f) ->
+      wf_asm_function f.
+
+  Ltac rewrite_hyps :=
+    repeat
+      match goal with
+        H1 : ?a = _, H2: ?a = _ |- _ => rewrite H1 in H2; inv H2
+      end.
+
+
+  Lemma group_progress:
+    forall rs s1
+      (SAFE : safe (RawAsm.semantics prog rs) s1),
+      (exists r, final_state s1 r) \/ (exists t s2, step (Genv.globalenv prog) s1 t s2).
+  Proof.
+    intros.
+    destruct (SAFE _  (star_refl _ _ _)) as [(r & FS)|(t & s2 & STEP)].
+    eauto.
+    destruct (pc_at ge s1) as [[[f i]|ef]|] eqn:PCs.
+    - destruct (is_call_dec (rs_state s1) i) as [CALL|NOTCALL].
+      + (* it's a call instruction : the next step is going to be either an external function or a Pallocframe. *)
+        simpl in STEP.
+        exploit step_internal; eauto. intro IB; inv IB; inv CALL. intros (EI & T0). subst.
+        destruct (SAFE _ (star_one _ _ _ _ _ STEP)) as [(r & FS)|(t & s3 & STEP2)].
+        * inv FS. simpl in EI.
+          inv CALL; simpl in EI; repeat destr_in EI.
+          -- simpl_regs_in H. unfold Genv.symbol_address in H. repeat destr_in H.
+          -- simpl_regs_in H. rewrite H in H1. inv H1.
+        * simpl in STEP2.
+          assert (exists b f', Genv.find_funct_ptr ge b = Some f' /\
+                          rs_state s2 PC = Vptr b Ptrofs.zero).
+          {
+            inv CALL; simpl in EI; repeat destr_in EI.
+            - unfold pc_at in PCs; repeat destr_in PCs; simpl in *; subst.
+              eapply wf_asm_call_target_exists in Heqo0; eauto.
+              destruct Heqo0 as (bf & f' & SA & FFP).
+              inv STEP2; simpl in *; subst; simpl_regs; simpl_regs_in H0; eauto.
+            - simpl_regs. rewrite H in *. simpl in Heqo. destr_in Heqo. eauto.
+          }
+          destruct H as (b & f' & FFP & PC2).
+          inversion STEP2; subst.
+          -- simpl in *. rewrite_hyps.
+             right; exists E0, (State rs' m').
+             eapply step_call_internal.  5: apply STEP. 5: apply STEP2. eauto.
+             unfold pc_at. rewrite PC2. rewrite H0, H1. eauto. eauto.
+             eapply wf_asm_alloc_at_beginning; eauto.
+          -- simpl in *. rewrite_hyps.
+             eapply wf_asm_alloc_at_beginning in H1; eauto. inv H1.
+          -- simpl in PC2. rewrite_hyps.
+             right; eexists t, (State _ m').
+             eapply step_call_external.  4: apply STEP. 4: apply STEP2. eauto. eauto.
+             unfold pc_at. rewrite PC2. rewrite H0. eauto. 
+      + (* not a call, free ? *)
+        destruct (is_free_dec i) as [(sz & ISFREE)|NISFREE].
+        * inversion ISFREE; subst. clear NOTCALL.
+          exploit step_internal; eauto. intro IB; inv IB. intros (EI & T0). subst.
+
+          destruct (SAFE _ (star_one _ _ _ _ _ STEP)) as [(r & FS)|(t & s3 & STEP2)].
+          -- inv FS. simpl in EI. repeat destr_in EI.
+             unfold pc_at in PCs. repeat destr_in PCs.
+             rewrite Asmgenproof0.nextinstr_pc in H.
+             simpl_regs_in H. simpl in H. rewrite Heqv0 in H. simpl in H. inv H.
+          -- unfold pc_at in PCs. repeat destr_in PCs.
+             destruct (wf_asm_after_freeframe _ (wf_asm_prog _ _ Heqo) _ _ _ Heqo0 ISFREE) as (SZ & i0 & FI0 & SPECi0). subst.
+             simpl in EI. repeat destr_in EI.
+             assert (t = E0).
+             {
+               inv STEP2; auto; unfold ge in *; simpl in *; subst; rewrite_hyps.
+               repeat simpl_regs_in H. rewrite Heqv in H; simpl in H; inv H.
+               unfold ge in *; simpl in *; subst; rewrite_hyps.
+               destruct SPECi0 as [A|A]; inv A.
+               repeat simpl_regs_in H. rewrite Heqv in H; simpl in H; inv H. congruence.
+             }
+             subst.
+             destruct SPECi0 as [RET | JMP].
+             ++ subst. right.
+                eexists _, _; eapply step_free_ret. 4: apply STEP. 4: apply STEP2.
+                simpl. fold ge. rewrite Heqv, Heqo, Heqo0. eauto.
+                unfold pc_at. destr. simpl in *; subst. 
+                rewrite Asmgenproof0.nextinstr_pc.
+                simpl_regs. rewrite Heqv. simpl. fold ge; rewrite Heqo. rewrite FI0. eauto.
+                constructor.
+             ++ destruct (SAFE _ (star_two _ _ _ _ _ _ _ STEP STEP2 eq_refl)) as [(ret & FS)|(t & s4 & STEP3)].
+                ** inv FS.
+
+
+                
+
+                rewrite FI0 in H2.
+                eexists _, _; eapply step_call_internal. 5: apply STEP. 5: apply STEP2.
+
+
+        * simpl in STEP2.
+          assert (exists b f', Genv.find_funct_ptr ge b = Some f' /\
+                          rs_state s2 PC = Vptr b Ptrofs.zero).
+          {
+            inv CALL; simpl in EI; repeat destr_in EI.
+            - unfold pc_at in PCs; repeat destr_in PCs; simpl in *; subst.
+              eapply wf_asm_call_target_exists in Heqo0; eauto.
+              destruct Heqo0 as (bf & f' & SA & FFP).
+              inv STEP2; simpl in *; subst; simpl_regs; simpl_regs_in H0; eauto.
+            - simpl_regs. rewrite H in *. simpl in Heqo. destr_in Heqo. eauto.
+          }
+          destruct H as (b & f' & FFP & PC2).
+          inversion STEP2; subst.
+          -- simpl in *. rewrite_hyps.
+             right; exists E0, (State rs' m').
+             eapply step_call_internal.  5: apply STEP. 5: apply STEP2. eauto.
+             unfold pc_at. rewrite PC2. rewrite H0, H1. eauto. eauto.
+             eapply wf_asm_alloc_at_beginning; eauto.
+          -- simpl in *. rewrite_hyps.
+             eapply wf_asm_alloc_at_beginning in H1; eauto. inv H1.
+          -- simpl in PC2. rewrite_hyps.
+             right; eexists t, (State _ m').
+             eapply step_call_external.  4: apply STEP. 4: apply STEP2. eauto. eauto.
+             unfold pc_at. rewrite PC2. rewrite H0. eauto. 
+
+  Qed.
+
+  Theorem group_correct:
+    forall rs,
+      backward_simulation (RawAsm.semantics prog rs) (semantics prog rs).
+  Proof.
+    intro rs.
+    eapply backward_simulation_plus with (match_states := fun (s1 s2: Asm.state) => s1 = s2).
+    - reflexivity.
+    - intros; eauto.
+    - simpl; intros s1 s2 I1 I2. eauto.
+    - intros; subst. auto.
+    - simpl; intros s1 s2 A SAFE; subst.
+      edestruct SAFE; eauto. apply star_refl.
+      destruct H as (t & s'' & STEP). simpl in *.
+      eapply group_progress; eauto.
+    - simpl; intros s2 t s2' STEP s1 EQ SAFE. subst.
+      eexists; split; eauto.
+      eapply step_correct; eauto.
+  Qed.
+
+End SIMU.
